Merge set language

main.py
@@ -1,0 +1,252 @@
+import sys
+import time
+
+import lark_parser
+from lark_parser import Lark_StandAlone, Transformer, v_args
+
+from lang import *
+
+@v_args(inline=True)
+class LangTransformer(Transformer):
+    var_tok = str
+    prop_val_tok = str
+    escaped_str = lambda self, v: str(v[1:-1]).replace('\\n', '\n').replace('\\r', '\r').replace('\\t', '\t') # Remove the quotes, which are the first and last characters
+
+    def int_tok(self, const):
+        if const.type != "INT":
+            raise Exception("Constants need to be integers: " + const)
+        return int(const.value)
+
+    # These functions exist because the two forms of ge and le have different numbers of symbols; these standardize it
+    def elim_ge(self, *args):
+        return '>='
+
+    def elim_le(self, *args):
+        return '<='
+
+    def elim_ne(self, *args):
+        return '!='
+
+    def var_ref(self, name):
+        return VarRef(str(name[0]))
+
+    def hint(self, a, b):
+        return Hint(a, b)
+
+    def ignore_singleton(f):
+        def go(self, *args):
+            if len(args) == 1:
+                return args[0]
+            else:
+                return f(*args)
+        return go
+
+    def parse_op(op_name, op):
+        def go(*args):
+            return BinArithOp(op_name, op, *args)
+        return go
+
+    start = lambda self, *args: list(args)
+
+    praline_add = ignore_singleton(parse_op('Add', add))
+    praline_sub = ignore_singleton(parse_op('Sub', sub))
+    praline_mul = ignore_singleton(parse_op('Mul', mul))
+    praline_div = ignore_singleton(parse_op('Div', divide))
+    praline_mod = ignore_singleton(parse_op('Mod', mod))
+
+    def section(self):
+        return Section()
+
+    def praline_string(self, s):
+        return Str(s)
+
+    praline_exp = ignore_singleton(Exp)
+    def elem(self, arg):
+        x, domain = arg
+        return Elem(x, domain)
+
+    def seq_def(self, lhs, rhs):
+        return lhs, rhs
+
+    def sequence(self, sym, *defs):
+        return Sequence(list(defs))
+
+    or_op = ignore_singleton(lambda *args: reduce(lambda a, b: Operator(a, 'or', operators['or'], b), args))
+    and_op = ignore_singleton(lambda *args: reduce(lambda a, b: Operator(a, 'and', operators['or'], b), args))
+
+    def image(self, f, arg):
+        return Image(f, arg)
+
+    def list(self, *args):
+        return List(*args)
+
+    def lambda_fun(self, *args):
+        args = list(args)
+        return Function(args[:-1], args[-1])
+
+    def if_stmt(self, cond, t, e):
+        return IfThenElse(cond, t, e)
+
+    def praline_app(self, func, *args):
+        return App(func, *args)
+
+    praline_factorial = Factorial
+    def praline_int(self, val):
+        return Num(val)
+
+    def operator(self, lhs, op, rhs):
+        return Operator(lhs, op, operators.get(op), rhs)
+
+    def praline_var(self, name):
+        return VarRef(str(name))
+
+    def operator_sym(self, sym):
+        return str(sym)
+
+    def praline_true(self):
+        return Num(1)
+
+    def praline_false(self):
+        return Num(0)
+
+    def varlist(self, *args):
+        return [ VarRef(x) for x in args ]
+
+    def quant_qual(self, *args):
+        return list(args)
+
+    def forall(self, sym, vs, body):
+        return Forall(vs, body)
+
+    def exists(self, sym, vs, body):
+        return Exists(vs, body)
+
+    def complement(self, sym, t):
+        return Complement(t)
+
+    def finset(self, *elems):
+        return FinSet(*elems)
+
+    def let_match(self, pat, t, body):
+        return LetBind(pat, t, body)
+
+    def comp_set(self, quant, sym, *preds):
+        orig_quant = quant
+
+        build_comp = True
+        if not isinstance(quant, Elem):
+            # This is actually a replacement set, and we need to find all the variables and their domains in the list of predicates
+            build_comp = False
+
+            quants = []
+            new_preds = []
+            for p in preds:
+                if isinstance(p, Elem):
+                    quants.append(p)
+                else:
+                    new_preds.append(p)
+
+            preds = new_preds
+            if len(quants) > 1:
+                quant = Elem(List(*[ q.x for q in quants ]), CartProd(*[ q.domain for q in quants ]))
+            else:
+                quant = quants[0]
+
+        if isinstance(quant.x, VarRef):
+            var_doms = [(quant.x, quant.domain)]
+        elif isinstance(quant.x, List):
+            if isinstance(quant.domain, Exp) and quant.domain.args[1].as_int() == len(quant.x.elems):
+                var_doms = [ (y, quant.domain.args[0]) for y in quant.x.elems ]
+            elif isinstance(quant.domain, CartProd):
+                var_doms = list(zip(quant.x.elems, quant.domain.sets))
+            else:
+                temp = VarRef(quant.fresh())
+                var_doms = [ (temp, quant.domain) ]
+                subs = { y.name: App(temp, Num(i)) for i, y in enumerate(quant.x.elems) }
+                preds = [ pred.substitute(subs) for pred in preds ]
+
+        if build_comp:
+            return ComprehensionSet(var_doms, list(preds)).simplify()
+        else:
+            if len(var_doms) > 1:
+                temp = VarRef(VarRef.fresh())
+                body = orig_quant.substitute({ y.name: App(temp, Num(i)) for i, (y, dom) in enumerate(var_doms) })
+                return Image(Function([var_doms[0][0]], body), ComprehensionSet(var_doms, list(preds))).simplify()
+            else:
+                return Image(Function([var_doms[0][0]], orig_quant), ComprehensionSet(var_doms, list(preds))).simplify()
+
+    def range_set(self, low, high):
+        return RangeSet(low, high, Num(1))
+
+    def range_set_step(self, low, step, high):
+        return RangeSet(low, high, BinArithOp('Sub', sub, step, low))
+
+    def definition(self, name, body):
+        return Definition(name, body)
+
+    def let_operator(self, name, body):
+        return Definition(VarRef(name), body)
+
+    def reduce(self, op, body):
+        if isinstance(op, VarRef):
+            return Reduce(op.name, operators.get(op.name), body)
+        else:
+            return Reduce(op, operators.get(op), body)
+
+    def reduce_sum(self, body):
+        return Reduce("++", operators.get('++'), body)
+
+parser = Lark_StandAlone(transformer=LangTransformer())
+
+if __name__ == '__main__':
+    default_env = {
+        'hints': {},
+        'ℕ': Naturals(),
+        'verbose': Num(0),
+        'ω': Num(OmegaOrd()),
+        'p': PrimeSeq(),
+        'choose': Builtin('choose', lambda a, args: args[0].eval(a).arbitrary(a)),
+        'gcd': Builtin('gcd', lambda a, args: Num(gcd(args[0].eval(a).as_int(), args[1].eval(a).as_int()))),
+        'next': Builtin('next', lambda a, args: args[0].eval(a).next_elem(args[1].eval(a), a)),
+        'card': Builtin('card', lambda a, args: args[0].eval(a).cardinality(a)),
+        'reverse': Builtin('reverse', lambda a, args: List(*args[0].eval(a).elems[::-1])),
+        'set': Builtin('set', lambda a, args: FinSet(*args[0].eval(a).enumerate(a))),
+        'list': Builtin('list', lambda a, args: List(*args[0].eval(a).enumerate(a))),
+        'num': Builtin('num', lambda a, args: Num(args[0].eval(a).as_rat().n)),
+        'denom': Builtin('denom', lambda a, args: Num(args[0].eval(a).as_rat().d)),
+        'min_elem': Builtin('min_elem', lambda a, args: args[0].eval(a).min_elem(a)),
+        'cache': Builtin('cache', lambda a, args: CachedSet(args[0].eval(a).val, args[1].eval(a))),
+        'sequence': Builtin('sequence', lambda a, args: SetSequence(args[0].eval(a)).eval(a)),
+        'cached_elements': Builtin('cached_elements', lambda a, args: FinSet(*args[0].eval(a).known_elements)),
+        '⋃': Builtin('⋃', lambda a, args: Union(list(args[0].eval(a).enumerate(a))).eval(a)),
+        '⋂': Builtin('⋂', lambda a, args: Union(list(args[0].eval(a).enumerate(a))).eval(a)),
+        'sort': Builtin('sort', lambda a, args: List(*sorted(list(val.enumerate(a))))),
+        'n_smallest': Builtin('n_smallest', n_smallest),
+        'cf': Builtin('cf', eval_cf),
+        'print': Builtin('print', print_val),
+        'μ': Builtin('μ', minimize),
+        'group': Builtin('group', group),
+    }
+
+    sys.setrecursionlimit(10000)
+
+    with open(sys.argv[1]) as f:
+        parsed = parser.parse(f.read())
+
+    all_start = time.time()
+    for stmt in parsed:
+        print('>', str(stmt))
+        if isinstance(stmt, lark_parser.Tree):
+            print('no_eval')
+        else:
+            start = time.time()
+            res = stmt.eval(default_env)
+            if res is not None:
+                print(str(res))
+            end = time.time()
+            if not isinstance(stmt, Definition):
+                print('Elapsed: {:.3f}'.format(end - start))
+    all_end = time.time()
+
+    print('Total elapsed: {:.3f}'.format(all_end - all_start))
+
