math.s
@@ -1,0 +1,130 @@
+Let '++' := (a,b) |-> a + b .
+Let '--' := (a,b) |-> a - b .
+Let '**' := (a,b) |-> a * b .
+Let '|' := (a,b) |-> b % a = 0 .
+
+2 + 2!
+
+Let max := X |-> choose({ x ∈ X : ∀y ∈ X . x ≥ y }) .
+Let min := X |-> choose({ x ∈ X : ∀y ∈ X . x ≤ y }) .
+Let minℕ := X |-> μ(x |-> x ∈ X) .
+
+minℕ({100...500})
+
+// choose(ℕ)
+∀x ∈ {1...100} . x + 2 < 10000
+choose({ x ∈ ℕ : x < 10 })
+num[ {1, 1/2, 1/4} ]
+cf([1,1,1,1,1])
+
+// if 1 = 1 then 2 else 0
+
+Sequence:
+    f(0) := 0;
+    f(1) := 1;
+    f(n) := f(n-1) + f(n-2) .
+
+f(12)
+
+Let Π := X |-> if X = {} then 1 else ** Σ X .
+
+// Project Euler 1
+Σ { x ∈ {1...999} : 3 | x or 5 | x }
+
+// Project Euler 2
+Let fib := n |-> num(cf((n |-> 1)[list({1...n})])) .
+Σ { x ∈ fib[{1...50}] : x < 4*10^6 and 2 | x }
+
+// Project Euler 3
+Let divisors := n |-> { d ∈ {1...n} : d | n } .
+// Let smallest_div := n |-> if n = 1 then 1 else μ(d |-> (d + 2) | n) + 2 .
+Let smallest_div := n |-> if n <= 1 then 1 else p(μ(k |-> p(k) | n)) .
+// Let is_prime := n |-> n > 1 and smallest_div(n) = n .
+smallest_div(42)
+
+Let int_sqrt := n |-> μ(m |-> m^2 >= n) .
+int_sqrt(10)
+Let is_prime := n |-> n = 2 or (n > 1 and ((not (2 | n)) and (not (exists m ∈ {3,5...int_sqrt(n)} . m | n)))) .
+
+Let primes := cache("primes", { n ∈ ℕ : is_prime(n) }) .
+min_elem(primes)
+
+choose(primes)
+// next(primes, 2)
+n_smallest(100, primes)
+
+Let factors := n |-> i |->
+    if i = 0
+    then smallest_div(n)
+    else smallest_div(n / Π((factors(n))[list({0...i-1})])) .
+// Let factor := n |-> (factors(n))[list({0...μ(m |-> (factors(n))(m + 1) = 1)})] .
+
+Let factor := n |->
+    if smallest_div(n) = n
+    then [n]
+    else [smallest_div(n)] @ factor(n / smallest_div(n)) .
+
+Hint(factor, "finite"). // Currently doesn't do anything
+max(factor(600851475143))
+
+// Project Euler 4
+Let int_log := n |-> μ(m |-> n / 10^m < 10) .
+Let nth_dig := n |-> i |-> (n / 10^(int_log(n) - i)) % 10 .
+Let digits := n |-> (nth_dig(n))[list({0...int_log(n)})] .
+Let is_palindrome := n |-> digits(n) = reverse(digits(n)) .
+
+// max({ n ∈ Π[{10...99}^2] : is_palindrome(n) })
+// max({ n ∈ Π[{100...999}^2] : is_palindrome(n) })
+// max({ n ∈ Π[{900...999}^2] : is_palindrome(n) })
+
+// Project Euler 5
+Let lcm := (a,b) |-> (a * b) / gcd(a,b) .
+lcm Σ {1...20}
+
+// Project Euler 6
+Let square := n |-> n^2 .
+square(Σ {1...100}) - (Σ square[{1...100}])
+
+// Project Euler 7
+// This is convenient and slick, but **way** slower than the builtin prime generator, which is just a sieve of eratosthenes
+// Let p := sequence(primes) .
+p(10000)
+
+// Project Euler 9
+let [a,b] := [1,2] in a + b
+card(ℕ)
+
+// { [a,b,c] ∈ {1...1000}^3 : a < b, b < c, c = 1000 - a - b, a^2 + b^2 = c^2 }
+
+// Project Euler 10:
+Section
+
+// Σ p[{0...μ(n |-> p(n) > 2000000)}]
+
+// TODO: Would be nice to be able to write this
+// Σ { p ∈ primes : p < 2000000 }
+
+// Project Euler 11:
+Let Tri := n |-> n*(n+1)/2 .
+Let factor_pow := n |-> { [p, μ(k |-> not (p^k | n)) - 1] : p ∈ factor(n) } .
+// Let d := n |-> card(divisors(n)) .
+// The below uses the prime factorization and is much faster.
+Let d := n |-> Π((p |-> p(1) + 1)[list(factor_pow(n))]) .
+// Tri(μ(n |-> d(Tri(n + 2)) > 500) + 2)
+
+// TODO: How is this not faster?
+Let dTri := n |-> if 2 | n then d(num(n / 2)) * d(n + 1) else d(n) * d(num((n + 1) / 2)) .
+// Tri(μ(n |-> dTri(n + 2) > 500) + 2)
+
+// Project Euler 12
+Let collatz := n |->
+    if n = 1 then [1]
+    else [n] @ collatz(if 2 | n then n / 2 else 3*n + 1) .
+
+Let collatzSteps := n |->
+    if n = 1 then 0
+    else 1 + collatzSteps(if 2 | n then n / 2 else 3*n + 1) .
+
+// { [n, card(collatz(n)) ] : n ∈ {1,3...10000} }
+{ [n, collatzSteps(n) ] : n ∈ {1,3...10000} }
+
